Test/comp/UnicodeStrings.dfy
@@ -2,7 +2,14 @@
 // RUN: %baredafny run --no-verify --unicode-char --target:cs "%s" %args >> "%t"
 // RUN: %diff "%s.expect" "%t"
 
+newtype uint32 = x: int | 0 <= x < 0x1_0000_0000
+newtype int32 = x: int | -0x8000_0000 <= x < 0x8000_0000
+
 method Main(args: seq<string>) {
   var trickyString := "Dafny is just so " + [0x1F60E as char];
   print trickyString, "\n";
+
+  var s := "Ceci n'est pas une string";
+  var notAString := seq(|s|, i requires 0 <= i < |s| => s[i] as int32);
+  print notAString, "\n";
 }
